1. The function BITWISE is defined in a different manner -- all dependent proofs are updated.    The old definition (which is more efficient for execution, but is not so easy to reason about) is poved to be equivalent with BITWISE_EVAL. 2. The theorem BIT_BITS_THM is generalised with a lower bound.

src/word32/word32Lib.sml
@@ -20,7 +20,7 @@ fun armword_rws () =
       REDUCE_RULE ONE_COMP_EVAL2,
       REDUCE_RULE TWO_COMP_EVAL2,
       SUBw_def,
-      REWRITE_RULE [LSB_ODD] BITWISE_EVAL2,
+      BITWISE_EVAL2,
       AND_EVAL2,
       OR_EVAL2,
       EOR_EVAL2,
