src/word32/bitsScript.sml
@@ -12,8 +12,6 @@ val _ = new_theory "bits";
 
 (* -------------------------------------------------------- *)
 
-val DIV2_def        = Define `DIV2 n = n DIV 2`;
-
 val TIMES_2EXP_def  = Define `TIMES_2EXP x n = n * 2 EXP x`;
 
 val DIV_2EXP_def    = Define `DIV_2EXP x n = n DIV 2 EXP x`;
@@ -30,14 +28,13 @@ val BIT_def         = Define `BIT b n = (BITS b b n = 1)`;
  
 val SLICE_def       = Define `SLICE h l n = MOD_2EXP (SUC h) n - MOD_2EXP l n`;
  
-val LSB_def         = Define`LSB = BIT 0`;
+val LSB_def         = Define `LSB = BIT 0`;
 
-val BITWISE_def = 
+val BITWISE_def =
  Define
-   `(BITWISE 0 op x y = 0) 
- /\ (BITWISE (SUC n) op x y = 
-       let r = (BITWISE n op (x DIV 2) (y DIV 2)) 
-       in if op (LSB x) (LSB y) then r + r + 1 else r + r)`;
+   `(BITWISE 0 op x y = 0)
+ /\ (BITWISE (SUC n) op x y =
+         BITWISE n op x y + SET (op (BIT n x) (BIT n y)) n)`;
 
 (* -------------------------------------------------------- *)
 (* -------------------------------------------------------- *)
@@ -211,8 +208,6 @@ val ODD_MOD2_LEM = store_thm("ODD_MOD2_LEM",
 
 (* -------------------------------------------------------- *)
 
-(* -------------------------------------------------------- *)
-
 val DIV1 = save_thm("DIV1",REDUCE_RULE DIV_ONE);
 
 val LSB_ODD = store_thm("LSB_ODD",
@@ -222,87 +217,6 @@ val LSB_ODD = store_thm("LSB_ODD",
 );
 
 (* -------------------------------------------------------- *)
-
-val LESS_MULT_MONO_SPEC = GEN_ALL (REWRITE_RULE [SYM TWO] 
-                                   (SPECL [`m`,`i`,`1`] LESS_MULT_MONO));
- 
-val LESS_MULT_MONO_SPEC2 = prove(
-  `!a b. a < b ==> 2 * a + 1 < 2 * b`,
-  RW_TAC arith_ss []
-);
-
-val ADD_DIV_ADD_DIV2 = save_thm("ADD_DIV_ADD_DIV2",
-  ONCE_REWRITE_RULE [MULT_COMM] 
-    (SIMP_RULE arith_ss [] (SPEC `2` ADD_DIV_ADD_DIV))
-);
-
-val ADD_DIV_ADD_DIV3 = save_thm("ADD_DIV_ADD_DIV3",
-  ONCE_REWRITE_RULE [ADD_COMM] ADD_DIV_ADD_DIV2
-);
-
-val BIT_DIV2 = store_thm("BIT_DIV2",
-  `!i. BIT n (i DIV 2) = BIT (SUC n) i`,
-  RW_TAC arith_ss [BIT_def,BITS_THM,EXP,ZERO_LT_TWOEXP,DIV_DIV_DIV_MULT]
-);
-
-val BITWISE_LT_2EXP = store_thm("BITWISE_LT_2EXP",
-  `!n op a b. BITWISE n op a b < 2 EXP n`,
-  Induct_on `n`
-    THEN REPEAT STRIP_TAC
-    THENL [
-      SIMP_TAC arith_ss [BITWISE_def],
-      FULL_SIMP_TAC arith_ss [BITWISE_def,EXP]
-        THEN RW_TAC arith_ss [LESS_MULT_MONO_SPEC,LESS_MULT_MONO_SPEC2]
-    ]
-);
-
-val BITWISE_THM = store_thm("BITWISE_THM",
-  `!x n op a b. x < n ==> (BIT x (BITWISE n op a b) = op (BIT x a) (BIT x b))`,
-  Induct_on `n`
-    THENL [
-      RW_TAC arith_ss [],
-      Induct_on `x`
-        THENL [
-           RW_TAC arith_ss [BITWISE_def,LSB_def]
-             THEN SIMP_TAC arith_ss [BIT_def,BITS2_THM,EXP,
-                                      ONCE_REWRITE_RULE [MULT_COMM] MOD_MULT,
-                                      ONCE_REWRITE_RULE [MULT_COMM] MOD_EQ_0],
-           RW_TAC arith_ss [BITWISE_def,LSB_def]
-             THEN `BIT x (BITWISE n op (a DIV 2) (b DIV 2)) =
-                    op (BIT x (a DIV 2)) (BIT x (b DIV 2))` by PROVE_TAC []
-             THEN RULE_ASSUM_TAC (REWRITE_RULE [BIT_DIV2])
-             THEN POP_ASSUM (fn th => REWRITE_TAC [SYM th])
-             THEN SIMP_TAC arith_ss [GSYM BIT_DIV2,ADD_DIV_ADD_DIV3,
-                                      ONCE_REWRITE_RULE [MULT_COMM] MULT_DIV]
-         ]
-    ]
-);
-
-val BITWISE_COR = store_thm("BITWISE_COR",
-  `!x n op a b. 
-      x < n ==> 
-      op (BIT x a) (BIT x b) ==> 
-     ((BITWISE n op a b DIV 2 EXP x) MOD 2 = 1)`,
-  NTAC 6 STRIP_TAC
-    THEN IMP_RES_TAC BITWISE_THM
-    THEN NTAC 2 (WEAKEN_TAC (K true))
-    THEN POP_ASSUM (fn th => REWRITE_TAC [GSYM th])
-    THEN ASM_SIMP_TAC std_ss 
-    [BITS_THM,BIT_def,DIV1,EXP_1,DECIDE(Term`SUC x - x = 1`)]
-);
- 
-val BITWISE_NOT_COR = store_thm("BITWISE_NOT_COR",
-  `!x n op a b. 
-     x < n ==> 
-     ~op (BIT x a) (BIT x b) ==> 
-    ((BITWISE n op a b DIV 2 EXP x) MOD 2 = 0)`,
-  NTAC 6 STRIP_TAC
-    THEN IMP_RES_TAC BITWISE_THM
-    THEN NTAC 2 (WEAKEN_TAC (K true))
-    THEN POP_ASSUM (fn th => REWRITE_TAC [GSYM th])
-    THEN ASM_SIMP_TAC std_ss [BITS_THM,BIT_def,GSYM NOT_MOD2_LEM,DIV1,EXP_1,
-                              DECIDE(Term`SUC x - x = 1`)]
-);
 
 val DIV_MULT_THM = store_thm("DIV_MULT_THM",
   `!x n. n DIV 2 EXP x * 2 EXP x = n - n MOD 2 EXP x`,
@@ -336,6 +250,24 @@ val TWOEXP_MONO2 = store_thm("TWOEXP_MONO2",
     THEN FULL_SIMP_TAC arith_ss [GSYM NOT_LESS]
     THEN IMP_RES_TAC LESS_CASES_IMP
     THEN RW_TAC std_ss [TWOEXP_MONO,NOT_LESS,LESS_IMP_LESS_OR_EQ]
+);
+
+val LESS_EXP_MULT = store_thm("LESS_EXP_MULT",
+  `!a b. a < b ==> ?p. 2 EXP b = p * 2 EXP a`,
+  REPEAT STRIP_TAC
+    THEN IMP_RES_TAC LESS_ADD
+    THEN RULE_ASSUM_TAC (ONCE_REWRITE_RULE [SIMP_RULE arith_ss [] (SPEC `2` (GSYM EXP_INJECTIVE))])
+    THEN EXISTS_TAC `2 EXP p`
+    THEN FULL_SIMP_TAC arith_ss [EXP_ADD]
+);
+ 
+val LESS_EQ_EXP_MULT = store_thm("LESS_EQ_EXP_MULT",
+  `!a b. a <= b ==> ?p. 2 EXP b = p * 2 EXP a`,
+  REPEAT STRIP_TAC
+    THEN IMP_RES_TAC LESS_EQUAL_ADD
+    THEN RULE_ASSUM_TAC (ONCE_REWRITE_RULE [SIMP_RULE arith_ss [] (SPEC `2` (GSYM EXP_INJECTIVE))])
+    THEN EXISTS_TAC `2 EXP p`
+    THEN FULL_SIMP_TAC arith_ss [EXP_ADD,MULT_COMM]
 );
 
 (* -------------------------------------------------------- *)
@@ -429,6 +361,223 @@ val SLICE_COMP_THM = store_thm("SLICE_COMP_THM",
              (SLICE h (SUC m) n + SLICE m l n = SLICE h l n)`,
   RW_TAC std_ss 
      [SLICE_def,MOD_2EXP_def,MOD_2EXP_MONO,GSYM LESS_EQ_ADD_SUB,SUB_ADD]
+);
+
+(* -------------------------------------------------------- *)
+
+val SUC_SUB = SIMP_CONV arith_ss [ADD1] ``SUC a - a``;
+ 
+val NOT_BIT = store_thm("NOT_BIT",
+  `!n a. ~BIT n a = (BITS n n a = 0)`,
+  RW_TAC std_ss [BIT_def,BITS_THM,SUC_SUB,EXP_1,GSYM NOT_MOD2_LEM]
+);
+ 
+val NOT_BITS = store_thm("NOT_BITS",
+  `!n a. ~(BITS n n a = 0) = (BITS n n a = 1)`,
+  RW_TAC std_ss [GSYM NOT_BIT,GSYM BIT_def]
+);
+ 
+val BIT_SLICE = store_thm("BIT_SLICE",
+  `!n a b. (BIT n a = BIT n b) = (SLICE n n a = SLICE n n b)`,
+  REPEAT STRIP_TAC THEN EQ_TAC
+    THENL [
+      Cases_on `BIT n a`
+        THEN FULL_SIMP_TAC arith_ss [BIT_def,SLICE_THM]
+        THEN FULL_SIMP_TAC arith_ss [GSYM NOT_BITS],
+      Cases_on `BITS n n a = 1`
+        THEN Cases_on `BITS n n b = 1`
+        THEN FULL_SIMP_TAC arith_ss [BIT_def,SLICE_THM]
+        THEN FULL_SIMP_TAC arith_ss [GSYM NOT_BITS,MULT_CLAUSES,
+                                     REWRITE_RULE [GSYM NOT_ZERO_LT_ZERO] ZERO_LT_TWOEXP]
+    ]
+);
+
+val BITS_ZERO = store_thm("BITS_ZERO",
+  `!h l n. h < l ==> (BITS h l n = 0)`,
+  REPEAT STRIP_TAC
+    THEN IMP_RES_TAC LESS_ADD_1
+    THEN POP_ASSUM (fn th => REWRITE_TAC [th])
+    THEN ASSUME_TAC (REWRITE_RULE [EXP,SUB,SUB_EQUAL_0]
+                       (ONCE_REWRITE_RULE [SUB_PLUS]
+                          (REWRITE_RULE [ADD1] (SPECL [`h`,`h + 1 + p`,`n`] BITSLT_THM))))
+    THEN FULL_SIMP_TAC arith_ss []
+);
+ 
+val SUB_BITS = prove(
+  `!h l a b. (BITS (SUC h) l a = BITS (SUC h) l b) ==> (BITS h l a = BITS h l b)`,
+  REPEAT STRIP_TAC
+    THEN Cases_on `h < l`
+    THENL [
+      RW_TAC std_ss [BITS_ZERO],
+      RULE_ASSUM_TAC (REWRITE_RULE [NOT_LESS])
+        THEN POP_ASSUM (fn th =>
+               ONCE_REWRITE_TAC [GSYM (SIMP_RULE arith_ss [th,SUB_ADD]
+               (SPECL [`SUC h`,`l`,`h-l`,`0`] BITS_COMP_THM))])
+        THEN ASM_REWRITE_TAC []
+    ]
+);
+
+val DECEND_LEMMA = prove(
+  `!P l y.  (!x. l <= x /\ x <= SUC y ==> P x) ==> (!x. l <= x /\ x <= y ==> P x)`,
+  RW_TAC arith_ss []
+);
+ 
+(* |- !m n. m < SUC n ==> m <= n *)
+val LESS_LEMMA3 = REWRITE_RULE [ONCE_REWRITE_RULE [DISJ_COMM] (GSYM LESS_OR_EQ)] LESS_LEMMA1;
+
+val BITS_SUC = prove(
+  `!h l a. BITS (SUC h) l a = if l = SUC h then
+                                BITS (SUC h) l (SLICE (SUC h) (SUC h) a)
+                              else
+                                BITS (SUC h) l (SLICE (SUC h) (SUC h) a + BITS h l a * 2 EXP l)`,
+  REPEAT STRIP_TAC
+    THEN Cases_on `SUC h < l`
+    THENL [
+      RW_TAC std_ss [BITS_ZERO],
+      RULE_ASSUM_TAC (REWRITE_RULE [NOT_LESS])
+        THEN RW_TAC arith_ss [GSYM SLICE_THM,BITS_SLICE_THM]
+        THEN `l < SUC h` by ASM_SIMP_TAC arith_ss []
+        THEN IMP_RES_TAC LESS_LEMMA3
+        THEN ASM_SIMP_TAC std_ss [BITS_SLICE_THM,SIMP_RULE arith_ss [] (SPECL [`SUC h`,`h`] SLICE_COMP_THM)]
+      ]
+);
+
+val BIT_BITS_LEM = prove(
+  `!h l a b. l <= h ==> (BITS h l a = BITS h l b) ==> (BIT h a = BIT h b)`,
+  RW_TAC std_ss [BIT_SLICE,SLICE_THM]
+    THEN PAT_ASSUM `l <= h` (fn th =>
+               ONCE_REWRITE_TAC [GSYM (SIMP_RULE arith_ss [th,SUB_ADD]
+               (SPECL [`h`,`l`,`h-l`,`h-l`] BITS_COMP_THM))])
+    THEN ASM_REWRITE_TAC []
+);
+
+val BIT_BITS_THM = store_thm("BIT_BITS_THM",
+  `!h l a b. (!x. l <= x /\ x <= h ==> (BIT x a = BIT x b)) = (BITS h l a = BITS h l b)`,
+  Induct_on `h`
+    THEN REPEAT STRIP_TAC
+    THENL [
+      Cases_on `l = 0`
+        THEN RW_TAC arith_ss [BIT_SLICE,SLICE_THM,EXP,SPEC `0` BITS_ZERO,NOT_ZERO_LT_ZERO],
+      EQ_TAC THEN REPEAT STRIP_TAC
+        THENL [
+          ONCE_REWRITE_TAC [BITS_SUC]
+            THEN RW_TAC std_ss []
+            THENL [
+               POP_ASSUM (fn th => SIMP_TAC std_ss [SIMP_RULE arith_ss [BIT_SLICE] (SPEC `SUC h` th)]),
+               Cases_on `SUC h < l`
+                 THENL [
+                   RW_TAC std_ss [BITS_ZERO],
+                   RULE_ASSUM_TAC (REWRITE_RULE [NOT_LESS])
+                     THEN PAT_ASSUM `!x. l <= x /\ x <= SUC h ==> (BIT x a = BIT x b)`
+                            (fn th => ASM_SIMP_TAC std_ss [SIMP_RULE arith_ss [BIT_SLICE] (SPEC `SUC h` th)]
+                            THEN ASSUME_TAC th)
+                     THEN POP_ASSUM (fn th => ASSUME_TAC (MATCH_MP
+                           (BETA_RULE (SPECL [`\x. BIT x a = BIT x b`,`l`,`h`] DECEND_LEMMA)) th))
+                     THEN PAT_ASSUM `!l a b.  (!x. l <= x /\ x <= h ==> (BIT x a = BIT x b)) =
+                                              (BITS h l a = BITS h l b)`
+                            (fn th => ASSUME_TAC (SPECL [`l`,`a`,`b`] th))
+                     THEN FULL_SIMP_TAC std_ss []
+                 ]
+            ],
+          IMP_RES_TAC SUB_BITS
+            THEN PAT_ASSUM `!l a b. (!x. l <= x /\ x <= h ==> (BIT x a = BIT x b)) =
+                                    (BITS h l a = BITS h l b)`
+                   (fn th => RULE_ASSUM_TAC (REWRITE_RULE [SYM (SPECL [`l`,`a`,`b`] th)]))
+            THEN Cases_on `x <= h`
+            THEN ASM_SIMP_TAC std_ss []
+            THEN `x = SUC h` by ASM_SIMP_TAC arith_ss []
+            THEN Cases_on `l = SUC h`
+            THENL [
+              FULL_SIMP_TAC std_ss [BIT_def],
+              `l <= SUC h` by ASM_SIMP_TAC arith_ss []
+                THEN POP_ASSUM (fn th => ASSUME_TAC (SIMP_RULE std_ss [th] (SPECL [`SUC h`,`l`,`a`,`b`] BIT_BITS_LEM)))
+                THEN FULL_SIMP_TAC std_ss []
+            ]
+        ]
+    ]
+);
+
+(* -------------------------------------------------------- *)
+
+val BITWISE_LT_2EXP = store_thm("BITWISE_LT_2EXP",
+  `!n op a b. BITWISE n op a b < 2 EXP n`,
+  Induct_on `n`
+    THEN RW_TAC std_ss [ADD_0,TIMES2,LESS_IMP_LESS_ADD,LESS_MONO_ADD,BITWISE_def,SET_def,EXP]
+    THEN REDUCE_TAC
+);
+
+val LESS_EXP_MULT2 = store_thm("LESS_EXP_MULT2",
+  `!a b. a < b ==> ?p. 2 EXP b = 2 EXP (p+1) * 2 EXP a`,
+  REPEAT STRIP_TAC
+    THEN IMP_RES_TAC LESS_ADD_1
+    THEN RULE_ASSUM_TAC (ONCE_REWRITE_RULE [SIMP_RULE arith_ss [] (SPEC `2` (GSYM EXP_INJECTIVE))])
+    THEN EXISTS_TAC `p`
+    THEN FULL_SIMP_TAC arith_ss [EXP_ADD,MULT_COMM]
+);
+
+val BITWISE_LEM = store_thm("BITWISE_THM",
+  `!n op a b. BIT n (BITWISE (SUC n) op a b) = op (BIT n a) (BIT n b)`,
+  RW_TAC arith_ss [SET_def,BITWISE_def,NOT_BIT]
+    THENL [
+       SIMP_TAC arith_ss [BIT_def,BITS_THM,SUC_SUB,SIMP_RULE arith_ss []
+                (SPEC `1` (SIMP_RULE std_ss [BITWISE_LT_2EXP]
+                   (SPECL [`2 EXP n`,`BITWISE n op a b`] DIV_MULT)))],
+       SIMP_TAC arith_ss [BITS_THM,LESS_DIV_EQ_ZERO,BITWISE_LT_2EXP,SUC_SUB]
+    ]
+);
+
+(* !x. 2 EXP (SUC x - x) = 2 *)
+val TWO_SUC_SUB = GEN_ALL (SIMP_CONV std_ss [SUC_SUB,EXP_1] ``2 EXP (SUC x - x)``);
+
+val LEFT_REWRITE_TAC = GEN_REWRITE_TAC (RATOR_CONV o DEPTH_CONV) empty_rewrites;
+
+val BITWISE_THM = store_thm("BITWISE_THM",
+  `!x n op a b. x < n ==> (BIT x (BITWISE n op a b) = op (BIT x a) (BIT x b))`,
+  Induct_on `n`
+    THEN REPEAT STRIP_TAC
+    THENL [
+      FULL_SIMP_TAC arith_ss [],
+      Cases_on `x = n`
+        THENL [
+           ASM_SIMP_TAC std_ss [BITWISE_LEM],
+           `x < n` by ASM_SIMP_TAC arith_ss []
+              THEN RW_TAC arith_ss [BITWISE_def,SET_def]
+              THEN LEFT_REWRITE_TAC [BIT_def]
+              THEN ASM_SIMP_TAC std_ss [BITS_THM]
+              THEN IMP_RES_TAC LESS_EXP_MULT2
+              THEN POP_ASSUM (K ALL_TAC)
+              THEN ASM_SIMP_TAC std_ss [ZERO_LT_TWOEXP,ADD_DIV_ADD_DIV,TWO_SUC_SUB,GSYM ADD1,EXP,
+                      ONCE_REWRITE_RULE [MULT_COMM] (REWRITE_RULE [DECIDE ``0 < 2``] (SPEC `2` MOD_TIMES))]
+              THEN SUBST_OCCS_TAC [([2],SYM (SPEC `x` TWO_SUC_SUB))]
+              THEN ASM_SIMP_TAC std_ss [GSYM BITS_THM,GSYM BIT_def]
+        ]
+    ]
+);
+
+val BITWISE_COR = store_thm("BITWISE_COR",
+  `!x n op a b. 
+      x < n ==> 
+      op (BIT x a) (BIT x b) ==> 
+     ((BITWISE n op a b DIV 2 EXP x) MOD 2 = 1)`,
+  NTAC 6 STRIP_TAC
+    THEN IMP_RES_TAC BITWISE_THM
+    THEN NTAC 2 (WEAKEN_TAC (K true))
+    THEN POP_ASSUM (fn th => REWRITE_TAC [GSYM th])
+    THEN ASM_SIMP_TAC std_ss 
+    [BITS_THM,BIT_def,DIV1,EXP_1,DECIDE(Term`SUC x - x = 1`)]
+);
+ 
+val BITWISE_NOT_COR = store_thm("BITWISE_NOT_COR",
+  `!x n op a b. 
+     x < n ==> 
+     ~op (BIT x a) (BIT x b) ==> 
+    ((BITWISE n op a b DIV 2 EXP x) MOD 2 = 0)`,
+  NTAC 6 STRIP_TAC
+    THEN IMP_RES_TAC BITWISE_THM
+    THEN NTAC 2 (WEAKEN_TAC (K true))
+    THEN POP_ASSUM (fn th => REWRITE_TAC [GSYM th])
+    THEN ASM_SIMP_TAC std_ss [BITS_THM,BIT_def,GSYM NOT_MOD2_LEM,DIV1,EXP_1,
+                              DECIDE(Term`SUC x - x = 1`)]
 );
 
 (* -------------------------------------------------------- *)
